correctness/RegexCorrectness/VM/Path/VMPath.lean
@@ -11,24 +11,25 @@ open String (Pos Iterator)
 
 namespace Regex.NFA
 
-inductive VMPath (nfa : NFA) (wf : nfa.WellFormed) : Iterator → Fin nfa.nodes.size → List (Nat × Pos) → Prop where
-  | init {it i update} (cls : nfa.εClosure' it ⟨nfa.start, wf.start_lt⟩ i update) :
-    VMPath nfa wf it i update
-  | more {i j k it update₁ update₂} (prev : VMPath nfa wf it i update₁) (step : nfa.CharStep it i j) (cls : nfa.εClosure' it.next j k update₂) :
-    VMPath nfa wf it.next k (update₁ ++ update₂)
+inductive VMPath (nfa : NFA) (wf : nfa.WellFormed) (it₀ : Iterator) : Iterator → Fin nfa.nodes.size → List (Nat × Pos) → Prop where
+  | init {it i update} (eqs : it.toString = it₀.toString) (le : it₀.pos ≤ it.pos) (cls : nfa.εClosure' it ⟨nfa.start, wf.start_lt⟩ i update) :
+    VMPath nfa wf it₀ it i update
+  | more {i j k it update₁ update₂ update₃} (prev : VMPath nfa wf it₀ it i update₁) (step : nfa.CharStep it i j) (cls : nfa.εClosure' it.next j k update₂)
+    (hupdate : update₃ = update₁ ++ update₂) :
+    VMPath nfa wf it₀ it.next k update₃
 
 namespace VMPath
 
-theorem eq_or_nfaPath {nfa : NFA} {wf it i update} (path : nfa.VMPath wf it i update) :
-  (i.val = nfa.start ∧ update = []) ∨
-  ∃ it₀, nfa.Path 0 nfa.start it₀ i it update := by
+theorem eq_or_nfaPath {nfa : NFA} {wf it₀ it i update} (path : nfa.VMPath wf it₀ it i update) :
+  (i.val = nfa.start ∧ update = [] ∧ it.toString = it₀.toString ∧ it₀.pos ≤ it.pos) ∨
+  ∃ its, its.toString = it₀.toString ∧ it₀.pos ≤ its.pos ∧ nfa.Path 0 nfa.start its i it update := by
   induction path with
-  | @init it i update cls =>
+  | @init itp i update eqs le cls =>
     simp [εClosure'_iff_path nfa wf] at cls
     cases cls with
-    | inl h => simp [←h.1, h.2]
-    | inr cls => exact .inr ⟨it, cls⟩
-  | @more i j k it update₁ update₂ prev step cls ih =>
+    | inl h => simp [←h.1, h.2, eqs, le, -Iterator.toString, -Iterator.pos]
+    | inr cls => exact .inr ⟨itp, eqs, le, cls⟩
+  | @more i j k it update₁ update₂ update₃ prev step cls equpdate ih =>
     have path₂ : nfa.Path 0 i it k it.next update₂ := by
       simp [εClosure'_iff_path nfa wf] at cls
       match cls with
@@ -38,14 +39,15 @@ theorem eq_or_nfaPath {nfa : NFA} {wf it i update} (path : nfa.VMPath wf it i up
       | .inr path => exact .more step path
 
     match ih with
-    | .inl ⟨eqi, equpdate⟩ =>
-      simp [←eqi, equpdate]
-      exact .inr ⟨it, path₂⟩
-    | .inr ⟨it₀, path₁⟩ => exact .inr ⟨it₀, path₁.trans path₂⟩
+    | .inl ⟨eqi, equpdate', eqs, le⟩ =>
+      simp [←eqi, equpdate']
+      simp [equpdate'] at equpdate
+      exact .inr ⟨it, eqs, le, equpdate ▸ path₂⟩
+    | .inr ⟨itp, eqs, le, path₁⟩ => exact .inr ⟨itp, eqs, le, equpdate ▸ path₁.trans path₂⟩
 
-theorem nfaPath_of_ne {nfa : NFA} {wf it i update} (path : nfa.VMPath wf it i update)
+theorem nfaPath_of_ne {nfa : NFA} {wf it₀ it i update} (path : nfa.VMPath wf it₀ it i update)
   (ne : i.val ≠ nfa.start):
-  ∃ it₀, nfa.Path 0 nfa.start it₀ i it update := by
+  ∃ its, its.toString = it₀.toString ∧ it₀.pos ≤ its.pos ∧ nfa.Path 0 nfa.start its i it update := by
   simpa [ne] using eq_or_nfaPath path
 
 end VMPath
@@ -58,14 +60,14 @@ namespace Regex.VM
 All states in `next.state` have a corresponding path from `nfa.start` to the state ending at `it`,
 and their updates are written to `next.updates` when necessary.
 -/
-def SearchState.Inv (nfa : NFA) (wf : nfa.WellFormed) (it : Iterator) (next : SearchState HistoryStrategy nfa) : Prop :=
+def SearchState.Inv (nfa : NFA) (wf : nfa.WellFormed) (it₀ it : Iterator) (next : SearchState HistoryStrategy nfa) : Prop :=
   ∀ i ∈ next.states,
     ∃ update,
-      nfa.VMPath wf it i update ∧
+      nfa.VMPath wf it₀ it i update ∧
       (εClosure.writeUpdate nfa[i] → next.updates[i] = update)
 
-theorem SearchState.Inv.of_empty {nfa wf it} {next : SearchState HistoryStrategy nfa} (h : next.states.isEmpty) :
-  next.Inv nfa wf it := by
+theorem SearchState.Inv.of_empty {nfa wf it₀ it} {next : SearchState HistoryStrategy nfa} (h : next.states.isEmpty) :
+  next.Inv nfa wf it₀ it := by
   intro i mem
   exact (SparseSet.not_mem_of_isEmpty h mem).elim
 
